almost there

src/Init/Data/List/Sort.lean
@@ -1,315 +1,324 @@
 import Lean
 
-section
-open Lean Elab Command
-
-syntax (name := timeCmd) "#time " command : command
-
-/--
-Time the elaboration of a command, and print the result (in milliseconds).
-
-Example usage:
-```
-set_option maxRecDepth 100000 in
-#time example : (List.range 500).length = 500 := rfl
-```
--/
-@[command_elab timeCmd] def timeCmdElab : CommandElab
-  | `(#time%$tk $stx:command) => do
-    let start ← IO.monoMsNow
-    elabCommand stx
-    logInfoAt tk m!"time: {(← IO.monoMsNow) - start}ms"
-  | _ => throwUnsupportedSyntax
-
-end
-
 namespace List
 
-def split : List α → List α × List α
-  | [] => ([], [])
-  | [a] => ([a], [])
-  | a :: b :: as =>
-    let (l, r) := split as
-    (a :: l, b :: r)
+def splitAt (n : Nat) (l : List α) : List α × List α := go l n [] where
+  /-- Auxiliary for `splitAt`: `splitAt.go xs n acc = (acc.reverse ++ take n xs, drop n xs)`
+  if `n < length xs`, else `(l, [])`. -/
+  go : List α → Nat → List α → List α × List α
+  | x :: xs, n+1, acc => go xs n (x :: acc)
+  | xs, _, acc => (acc.reverse, xs)
 
-@[simp] theorem split_nil : split ([] : List α) = ([], []) := rfl
-@[simp] theorem split_singleton (a : α) : split [a] = ([a], []) := rfl
-@[simp] theorem split_cons_cons (a b : α) (as : List α) : split (a :: b :: as) = (a :: (split as).1, b :: (split as).2) := rfl
+theorem splitAt_go (n : Nat) (l acc : List α) :
+    splitAt.go l n acc = (acc.reverse ++ l.take n, l.drop n) := by
+  induction l generalizing n acc with
+  | nil => simp [splitAt.go]
+  | cons x xs ih =>
+    cases n with
+    | zero => simp [splitAt.go]
+    | succ n =>
+      rw [splitAt.go, take_succ_cons, drop_succ_cons, ih n (x :: acc),
+        reverse_cons, append_assoc, singleton_append]
 
-theorem split_fst_length : (l : List α) → (split l).1.length = (l.length + 1) / 2
-  | [] | [_] | a :: b :: as => by simp [split, split_fst_length] <;> omega
+theorem splitAt_eq (n : Nat) (l : List α) : splitAt n l = (l.take n, l.drop n) := by
+  rw [splitAt, splitAt_go, reverse_nil, nil_append]
 
-theorem split_snd_length : (l : List α) → (split l).2.length = l.length / 2
-  | [] | [_] | a :: b :: as => by simp [split, split_snd_length] <;> omega
+namespace mergeSort
 
-def merge (lt : α → α → Bool) : List α → List α → List α
-  | [], ys => ys
-  | xs, [] => xs
-  | x :: xs, y :: ys =>
-    if lt x y then
-      x :: merge lt xs (y :: ys)
-    else
-      y :: merge lt (x :: xs) ys
+abbrev Vec (α : Type) (n : Nat) := { l : List α // l.length = n }
 
-@[simp] theorem merge_nil (lt : α → α → Bool) (xs : List α) : merge lt xs [] = xs := by
-  cases xs <;> simp [merge]
+def split (l : Vec α n) : Vec α ((n+1)/2) × Vec α (n/2) :=
+  let r := splitAt ((n+1)/2) l.1
+  (⟨r.1, by simp [r, splitAt_eq, l.2]; omega⟩, ⟨r.2, by simp [r, splitAt_eq, l.2]; omega⟩)
 
-def mergeSort (lt : α → α → Bool) : List α → List α
-  | [] => []
-  | [a] => [a]
-  | a :: b :: xs =>
-    let lr := split (a :: b :: xs)
-    have := split_fst_length xs
-    have := split_snd_length xs
-    merge lt (lr.1.mergeSort lt) (lr.2.mergeSort lt)
-  termination_by l => l.length
-
-theorem mem_merge (lt : α → α → Bool) {a : α} : (xs ys : List α) → a ∈ merge lt xs ys ↔ a ∈ xs ∨ a ∈ ys
-  | [], ys => by simp [merge]
-  | xs, [] => by simp [merge]
-  | x :: xs, y :: ys => by
-    simp [merge]
-    split <;> rename_i h
-    · simp only [mem_cons, mem_merge lt xs (y :: ys), or_assoc]
-    · simp only [mem_cons, mem_merge lt (x :: xs) ys, ← or_assoc]
-      apply or_congr_left
-      rw [or_comm (a := a = y), or_assoc, or_assoc]
-      apply or_congr_right
-      rw [or_comm]
-
-theorem mem_of_mem_split_fst {a : α} {l : List α} : a ∈ (split l).1 → a ∈ l := by
-  sorry
-theorem mem_of_mem_split_snd {a : α} {l : List α} : a ∈ (split l).2 → a ∈ l := by
-  sorry
-
-theorem split_fst_sublist (l : List α) : (split l).1 <+ l := by
-  sorry
-theorem split_snd_sublist (l : List α) : (split l).2 <+ l := by
-  sorry
-
-def sorted (lt : α → α → Bool) (xs : List α) : Prop := xs.Pairwise fun a b => !lt b a
-
-variable (lt : α → α → Bool)
-
-theorem split_fst_sorted : (l : List α) → sorted lt l → sorted lt (split l).1
-  | [], h => by simpa [split]
-  | [a], h => by simpa [split]
-  | a :: b :: as, h => by
-    simp [split]
-    constructor
-    · cases h
-      rename_i h
-      intro z m
-      exact h z (mem_cons.mpr (Or.inr (mem_of_mem_split_fst m)))
-    · cases h
-      rename_i h w
-      exact h.tail.sublist (split_fst_sublist as)
-
-theorem split_snd_sorted : (l : List α) → sorted lt l → sorted lt (split l).2
-  | [], h => by simpa [split]
-  | [a], h => by simp [split, sorted]
-  | a :: b :: as, h => by
-    simp [split]
-    constructor
-    · cases h
-      rename_i h
-      intro z m
-      sorry
-    · cases h
-      rename_i h w
-      exact h.tail.sublist (split_snd_sublist as)
-
-theorem merge_split_of_sorted : (l : List α) → sorted lt l → merge lt (split l).1 (split l).2 = l
-  | [], _ => sorry
-  | [a], _ => sorry
-  | a :: b :: as, h => by
-    simp [merge]
-    have := split_fst_length as
-    have := split_snd_length as
-    rw [if_pos]
-    sorry
-    sorry
-
-theorem merge_split_cons_of_sorted : (b : α) → (as : List α) → sorted lt (b :: as) → merge lt (split as).1 (b :: (split as).2) = b :: as := by
-  sorry
-
-
-section
-variable (antisymm : ∀ a b, lt a b → !lt b a) (trans : ∀ a b c, lt a b → lt b c → lt a c)
-    (total : ∀ a b, a ≠ b → !lt a b → lt b a)
-include antisymm trans total
-
-theorem merge_sorted :
-    {xs ys : List α} → sorted lt xs → sorted lt ys → sorted lt (merge lt xs ys)
-  | [], ys, _, h => by simpa [merge]
-  | xs, [], h, _ => by simpa [merge]
-  | x :: xs, y :: ys, h₁, h₂ => by
-    simp [merge]
-    split <;> rename_i xy
-    · constructor
-      · intro z m
-        simp only [Bool.not_eq_true']
-        simp [mem_merge] at m
-        rcases m with m | rfl | m
-        · have := rel_of_pairwise_cons h₁ m
-          apply Decidable.byContradiction
-          intro zx
-          specialize trans _ _ _ (by simpa using zx) xy
-          simp_all
-        · specialize antisymm x z
-          simp_all
-        · have := rel_of_pairwise_cons h₂ m
-          simp at this
-          specialize antisymm _ _ xy
-          apply Decidable.byContradiction
-          intro zx
-          specialize trans _ _ _ (by simpa using zx) xy
-          simp_all
-      · exact merge_sorted h₁.tail h₂
-    · constructor
-      · intro z m
-        simp only [Bool.not_eq_true']
-        simp [mem_merge] at m
-        rcases m with (rfl | m) | m
-        · simpa using xy
-        · have := rel_of_pairwise_cons h₁ m
-          apply Decidable.byContradiction
-          intro zy
-          by_cases xy' : x = y
-          · simp_all
-          · specialize total _ _ xy' (by simpa using xy)
-            specialize trans _ _ _ (by simpa using zy) total
-            simp_all
-        · have := rel_of_pairwise_cons h₂ m
-          apply Decidable.byContradiction
-          intro zy
-          simp_all
-      · exact merge_sorted h₁ h₂.tail
-
-theorem mergeSort_sorted : (xs : List α) → sorted lt (mergeSort lt xs)
-  | []
-  | [a] => by simp [mergeSort, sorted]
-  | a :: b :: xs => by
-    simp [mergeSort]
-    apply merge_sorted lt antisymm trans total
-    · have := split_fst_length xs
-      apply mergeSort_sorted
-    · have := split_snd_length xs
-      apply mergeSort_sorted
-termination_by l => l.length
-
-theorem mergeSort_eq_self_of_sorted : (xs : List α) → sorted lt xs → mergeSort lt xs = xs
-  | [], _ => sorry
-  | [a], _ => sorry
-  | a :: b :: xs, h => by
-    simp [mergeSort]
-    have := split_fst_length xs
-    have := split_snd_length xs
-    rw [mergeSort_eq_self_of_sorted]
-    rw [mergeSort_eq_self_of_sorted]
-    rw [merge, if_pos sorry, merge_split_cons_of_sorted]
-    exact h.tail
-    sorry
-    sorry
-  termination_by l => l.length
-
-theorem mergeSort_mergeSort (xs : List α) : mergeSort lt (mergeSort lt xs) = mergeSort lt xs :=
-  mergeSort_eq_self_of_sorted lt antisymm trans total (mergeSort lt xs) (mergeSort_sorted lt antisymm trans total xs)
-
-#eval! mergeSort (· < ·) [3, 1, 4, 1, 5, 9, 2, 6, 5, 3, 5]
-
--- Stack overflow at 10000.
-#eval! (mergeSort (· < ·) (List.range 1000)).length
-
-def splitRev (l : List α) : List α × List α :=
-  go l [] []
-where go : List α → List α → List α → List α × List α
-  | [], l₁, l₂ => (l₁, l₂)
-  | [a], l₁, l₂ => (a :: l₁, l₂)
-  | a :: b :: as, l₁, l₂ =>
-    go as (a :: l₁) (b :: l₂)
-
-#eval splitRev [1,2,3,4,5,6]
-
-theorem splitRev_go_fst_length : (l l₁ l₂ : List α) → (splitRev.go l l₁ l₂).1.length = (l.length + 1) / 2 + l₁.length
-| [], _, _
-| [_], _, _ => by simp [splitRev.go] <;> omega
-| a :: b :: as, l₁, l₂ => by
-  simp only [splitRev.go]
-  rw [splitRev_go_fst_length as (a :: l₁) (b :: l₂)]
-  simp
-  omega
-
-theorem splitRev_go_snd_length : (l l₁ l₂ : List α) → (splitRev.go l l₁ l₂).2.length = l.length / 2 + l₂.length
-| [], _, _
-| [_], _, _ => by simp [splitRev.go]
-| a :: b :: as, l₁, l₂ => by
-  simp only [splitRev.go]
-  have := splitRev_go_snd_length as (a :: l₁) (b :: l₂)
-  rw [this]
-  simp
-  omega
-
-theorem splitRev_go_fst_length_le (l l₁ l₂ : List α) : (splitRev.go l l₁ l₂).1.length ≤ l.length + l₁.length := by
-  have := splitRev_go_fst_length l l₁ l₂
-  omega
-
-theorem splitRev_go_snd_length_le (l l₁ l₂ : List α) : (splitRev.go l l₁ l₂).2.length ≤ l.length + l₂.length := by
-  have := splitRev_go_snd_length l l₁ l₂
-  omega
-
-@[simp] theorem splitRev_cons_cons_fst_length (a b : α) (as : List α) : (splitRev (a :: b :: as)).1.length = (splitRev as).1.length + 1 := by
-  simp [splitRev, splitRev_go_fst_length]
-  omega
-
-@[simp] theorem splitRev_cons_cons_snd_length (a b : α) (as : List α) : (splitRev (a :: b :: as)).2.length = (splitRev as).2.length + 1 := by
-  simp [splitRev, splitRev_go_snd_length]
-  omega
-
-theorem splitRev_fst_length_le (l : List α) : (splitRev l).1.length ≤ l.length := by
-  simp [splitRev]
-  have := splitRev_go_fst_length_le l [] []
-  simp at this
-  omega
-
-theorem splitRev_snd_length_le (l : List α) : (splitRev l).2.length ≤ l.length := by
-  simp [splitRev]
-  have := splitRev_go_snd_length_le l [] []
-  simp at this
-  omega
-
-def merge2 (s : α → α → Prop) [DecidableRel s] (l₁ l₂ : List α) : List α :=
+def merge (le : α → α → Bool) (l₁ l₂ : List α) : List α :=
   go l₁ l₂ []
 where go : List α → List α → List α → List α
   | [], l₂, acc => acc.reverse ++ l₂
   | l₁, [], acc => acc.reverse ++ l₁
   | x :: xs, y :: ys, acc =>
-    if s x y then
+    if le x y then
       go xs (y :: ys) (x :: acc)
     else
       go (x :: xs) ys (y :: acc)
 
-#eval merge2 (· < ·) [1, 3, 5] [2, 4, 6]
+end mergeSort
 
-def mergeSort2 (s : α → α → Prop) [DecidableRel s] : List α → List α
+open mergeSort
+
+def mergeSort (le : α → α → Bool) (l : List α) : List α :=
+  run ⟨l, rfl⟩
+where run : {n : Nat} → Vec α n → List α
+  | 0, ⟨[], _⟩ => []
+  | 1, ⟨[a], _⟩ => [a]
+  | n+2, xs =>
+    let (l, r) := split xs
+    merge le (run l) (run r)
+
+#eval mergeSort (· ≤ ·) [3, 1, 4, 1, 5, 9, 2, 6, 5, 3, 5]
+
+#eval mergeSort (fun x y => x/10 ≤ y/10) [3, 100 + 1, 4, 100 + 1, 5, 100 + 9, 2, 10 + 6, 5, 10 + 3, 5]
+
+abbrev Sorted (r : α → α → Bool) (xs : List α) : Prop := xs.Pairwise (fun x y => r x y)
+
+namespace mergeSort
+
+@[simp] theorem split_fst (l : Vec α n) : (split l).1 = ⟨l.1.take ((n+1)/2), by simp [split, splitAt_eq, l.2]; omega⟩ := by
+  simp [split, splitAt_eq]
+
+@[simp] theorem split_snd (l : Vec α n) : (split l).2 = ⟨l.1.drop ((n+1)/2), by simp [split, splitAt_eq, l.2]; omega⟩ := by
+  simp [split, splitAt_eq]
+
+theorem split_fst_append_split_snd (l : Vec α n) : (split l).1.1 ++ (split l).2.1 = l.1 := by
+  simp
+
+variable {le : α → α → Bool}
+
+def naiveMerge (lt : α → α → Bool) : List α → List α → List α
+  | [], ys => ys
+  | xs, [] => xs
+  | x :: xs, y :: ys =>
+    if lt x y then
+      x :: naiveMerge lt xs (y :: ys)
+    else
+      y :: naiveMerge lt (x :: xs) ys
+
+@[simp] theorem naiveMerge_nil_right (xs : List α) : naiveMerge le xs [] = xs := by
+  induction xs with
+  | nil => simp [naiveMerge]
+  | cons x xs ih => simp [naiveMerge, ih]
+
+theorem merge_go_eq_naiveMerge : merge.go le l₁ l₂ acc = acc.reverse ++ naiveMerge le l₁ l₂ := by
+  induction l₁ generalizing l₂ acc with
+  | nil => simp [merge.go, naiveMerge]
+  | cons x l₁ ih₁ =>
+    induction l₂ generalizing acc with
+    | nil => simp [merge.go, naiveMerge]
+    | cons y l₂ ih₂ =>
+      simp [merge.go, naiveMerge]
+      split <;> simp [ih₁, ih₂]
+
+theorem merge_eq_naiveMerge : merge le l₁ l₂ = naiveMerge le l₁ l₂ := by
+  simp [merge, merge_go_eq_naiveMerge]
+
+def naiveMergeSort (le : α → α → Bool) : List α → List α
   | [] => []
   | [a] => [a]
-  | a :: b :: xs  =>
-    let lr := splitRev (a :: b :: xs)
-    have := splitRev_fst_length_le xs
-    have := splitRev_snd_length_le xs
-    merge2 s (lr.1.mergeSort2 s) (lr.2.mergeSort2 s)
+  | a :: b :: xs =>
+    let lr := split ⟨a :: b :: xs, rfl⟩
+    have := by simpa using lr.2.2
+    have := by simpa using lr.1.2
+    naiveMerge le (naiveMergeSort le lr.1) (naiveMergeSort le lr.2)
 termination_by l => l.length
 
-#eval! mergeSort2 (· < ·) [3, 1, 4, 1, 5, 9, 2, 6, 5, 3, 5]
+theorem mergeSort_run_eq_naiveMergeSort : {n : Nat} → (l : Vec α n) → mergeSort.run le l = naiveMergeSort le l.1
+  | 0, ⟨[], _⟩
+  | 1, ⟨[a], _⟩ => by simp [run, naiveMergeSort]
+  | n+2, ⟨a :: b :: l, h⟩ => by
+    cases h
+    simp [run, naiveMergeSort]
+    rw [merge_eq_naiveMerge]
+    rw [mergeSort_run_eq_naiveMergeSort, mergeSort_run_eq_naiveMergeSort]
 
--- 1 * 10^6: 3.9ms
--- 2 * 10^6: 9.8ms
--- 3 * 10^6: 12.8s
--- #time
--- #eval! (mergeSort2 (· < ·) (List.range (3 * 10^6))).length
+theorem mergeSort_eq_naiveMergeSort : mergeSort le l = naiveMergeSort le l := by
+  rw [mergeSort, mergeSort_run_eq_naiveMergeSort]
 
--- crashes between 10^5 and 10^6
-#eval (Array.qsort (List.range (1 * 10^5)).toArray fun a b => a < b).size
+theorem mem_naiveMerge {a : α} {xs ys : List α} : a ∈ naiveMerge le xs ys ↔ a ∈ xs ∨ a ∈ ys := by
+  induction xs generalizing ys with
+  | nil => simp [naiveMerge]
+  | cons x xs ih =>
+    induction ys with
+    | nil => simp [naiveMerge]
+    | cons y ys ih =>
+      simp only [naiveMerge]
+      split <;> rename_i h
+      · simp_all [or_assoc]
+      · simp only [mem_cons, or_assoc, Bool.not_eq_true, ih, ← or_assoc]
+        apply or_congr_left
+        simp only [or_comm (a := a = y), or_assoc]
+
+theorem naiveMerge_sorted
+    (trans : ∀ {a b c : α}, le a b → le b c → le a c)
+    (total : ∀ {a b : α}, !le a b → le b a)
+    (l₁ l₂ : List α) (h₁ : l₁.Sorted le) (h₂ : l₂.Sorted le) : (naiveMerge le l₁ l₂).Sorted le := by
+  induction l₁ generalizing l₂ with
+  | nil => simpa only [naiveMerge]
+  | cons x l₁ ih₁ =>
+    induction l₂ with
+    | nil => simpa only [naiveMerge]
+    | cons y l₂ ih₂ =>
+      simp only [naiveMerge]
+      split <;> rename_i h
+      · apply Pairwise.cons
+        · intro z m
+          rw [mem_naiveMerge, mem_cons] at m
+          rcases m with (m|rfl|m)
+          · exact rel_of_pairwise_cons h₁ m
+          · exact h
+          · exact trans h (rel_of_pairwise_cons h₂ m)
+        · exact ih₁ _ h₁.tail h₂
+      · apply Pairwise.cons
+        · intro z m
+          rw [mem_naiveMerge, mem_cons] at m
+          rcases m with (⟨rfl|m⟩|m)
+          · exact total (by simpa using h)
+          · exact trans (total (by simpa using h)) (rel_of_pairwise_cons h₁ m)
+          · exact rel_of_pairwise_cons h₂ m
+        · exact ih₂ h₂.tail
+
+theorem naiveMergeSort_sorted
+    (trans : ∀ {a b c : α}, le a b → le b c → le a c)
+    (total : ∀ {a b : α}, !le a b → le b a) :
+    (l : List α) → (naiveMergeSort le l).Sorted le
+  | [] => by simp [naiveMergeSort]
+  | [a] => by simp [naiveMergeSort]
+  | a :: b :: xs => by
+    have : (split ⟨a :: b :: xs, rfl⟩).1.1.length < xs.length + 1 + 1 := by simp [split_fst]; omega
+    have : (split ⟨a :: b :: xs, rfl⟩).2.1.length < xs.length + 1 + 1 := by simp [split_snd]; omega
+    rw [naiveMergeSort]
+    apply naiveMerge_sorted @trans @total
+    apply naiveMergeSort_sorted trans total
+    apply naiveMergeSort_sorted trans total
+termination_by l => l.length
+
+theorem split_fst_sorted (l : Vec α n) (h : Sorted le l) : Sorted le (split l).1 := by
+  rw [split_fst]
+  exact h.take
+
+theorem split_snd_sorted (l : Vec α n) (h : Sorted le l) : Sorted le (split l).2 := by
+  rw [split_snd]
+  exact h.drop
+
+theorem split_fst_le_split_snd {l : Vec α n} (h : Sorted le l) :
+    ∀ a b, a ∈ (split l).1.1 → b ∈ (split l).2.1 → le a b := by
+  rw [split_fst, split_snd]
+  intro a b ma mb
+  exact h.rel_of_mem_take_of_mem_drop ma mb
+
+theorem naiveMerge_of_le : ∀ {xs ys : List α} (_ : ∀ a b, a ∈ xs → b ∈ ys → le a b),
+    naiveMerge le xs ys = xs ++ ys
+  | [], ys, _
+  | xs, [], _ => by simp [naiveMerge]
+  | x :: xs, y :: ys, h => by
+    simp only [naiveMerge, cons_append]
+    rw [if_pos, naiveMerge_of_le]
+    · intro a b ma mb
+      exact h a b (mem_cons_of_mem _ ma) mb
+    · exact h x y (mem_cons_self _ _) (mem_cons_self _ _)
+
+theorem naiveMergeSort_of_sorted : ∀ {l : List α} (_ : Sorted le l), naiveMergeSort le l = l
+  | [], _ => by simp [naiveMergeSort]
+  | [a], _ => by simp [naiveMergeSort]
+  | a :: b :: xs, h => by
+    have : (split ⟨a :: b :: xs, rfl⟩).1.1.length < xs.length + 1 + 1 := by simp [split_fst]; omega
+    have : (split ⟨a :: b :: xs, rfl⟩).2.1.length < xs.length + 1 + 1 := by simp [split_snd]; omega
+    rw [naiveMergeSort]
+    rw [naiveMergeSort_of_sorted (split_fst_sorted ⟨a :: b :: xs, rfl⟩ h)]
+    rw [naiveMergeSort_of_sorted (split_snd_sorted ⟨a :: b :: xs, rfl⟩ h)]
+    rw [naiveMerge_of_le (split_fst_le_split_snd h)]
+    rw [split_fst_append_split_snd]
+termination_by l => l.length
+
+def stable_le (le : α → α → Bool) (a b : Nat × α) : Bool :=
+  if le a.2 b.2 then if le b.2 a.2 then a.1 ≤ b.1 else true else false
+
+theorem split_cons_cons_enumFrom_fst (i : Nat) (l : List α) :
+    (split ⟨(i, a) :: (i+1, b) :: l.enumFrom (i+2), rfl⟩).1.1 =
+      (split ⟨a :: b :: l, rfl⟩).1.1.enumFrom i := by
+  simp_all
+  ext1 j
+  rw [getElem?_take]
+  rw [getElem?_enumFrom]
+  rw [getElem?_cons]
+  rw [take_cons (by omega), take_cons (α := α) (by omega), enumFrom_cons]
+  congr 1
+  induction l generalizing i with
+  | nil => simp
+  | cons c l ih =>
+    simp
+    rw [take_cons (by omega), take_cons (α := α) (by omega), enumFrom_cons]
+    congr 1
+    cases l with
+    | nil => simp
+    | cons d l =>
+
+theorem split_cons_cons_enumFrom_snd (i : Nat) (l : List α) :
+    (split ⟨(i, a) :: (i+1, b) :: l.enumFrom (i+2), rfl⟩).2.1 =
+      (split ⟨a :: b :: l, rfl⟩).2.1.enumFrom (i+(l.length+3)/2) := by
+  sorry
+
+theorem naiveMerge_stable : ∀ (xs ys) (h : ∀ x y, x ∈ xs → y ∈ ys → x.1 ≤ y.1),
+    (naiveMerge (stable_le le) xs ys).map (·.2) = naiveMerge le (xs.map (·.2)) (ys.map (·.2))
+  | [], ys, _ => by simp [naiveMerge]
+  | xs, [], _ => by simp [naiveMerge]
+  | (i, x) :: xs, (j, y) :: ys, h => by
+    simp only [naiveMerge, stable_le, map_cons]
+    split <;> rename_i w
+    · rw [if_pos]
+      simp
+      rw [naiveMerge_stable]
+      rw [map_cons]
+      sorry
+      sorry
+    · simp
+      rw [naiveMerge_stable, map_cons]
+      sorry
+
+-- TODO: replace this with a proof via `Perm`
+@[simp] theorem mem_naiveMergeSort {a : α} {l : List α} : a ∈ naiveMergeSort le l ↔ a ∈ l := by
+  sorry
+
+theorem naiveMergeSort_stable : ∀ {i : Nat} {l : List α},
+    (naiveMergeSort (stable_le le) (l.enumFrom i)).map (·.2) = naiveMergeSort le l
+  | _, []
+  | _, [a] => by simp [naiveMergeSort]
+  | _, a :: b :: xs => by
+    have : (split ⟨a :: b :: xs, rfl⟩).1.1.length < xs.length + 1 + 1 := by simp [split_fst]; omega
+    have : (split ⟨a :: b :: xs, rfl⟩).2.1.length < xs.length + 1 + 1 := by simp [split_snd]; omega
+    simp only [naiveMergeSort, enumFrom]
+    rw [split_cons_cons_enumFrom_fst]
+    rw [split_cons_cons_enumFrom_snd]
+    rw [naiveMerge_stable]
+    · rw [naiveMergeSort_stable, naiveMergeSort_stable]
+    · simp only [mem_naiveMergeSort, Prod.forall]
+      intros j x k y mx my
+      have := mem_enumFrom mx
+      have := mem_enumFrom my
+      simp_all
+      omega
+termination_by _ l => l.length
+
+end mergeSort
+
+theorem mergeSort_sorted
+    (trans : ∀ {a b c : α}, le a b → le b c → le a c)
+    (total : ∀ {a b : α}, !le a b → le b a)
+    (l : List α) : (mergeSort le l).Sorted le := by
+  rw [mergeSort_eq_naiveMergeSort]
+  apply naiveMergeSort_sorted @trans @total
+
+theorem mergeSort_of_sorted (h : Sorted le l) : mergeSort le l = l := by
+  rw [mergeSort_eq_naiveMergeSort]
+  apply naiveMergeSort_of_sorted h
+
+/--
+This merge sort algorithm is "stable",
+in the sense that breaking ties in the ordering function using the position in the list
+has no effect on the output.
+
+That is, elements which are equal with respect to the ordering function will remain
+in the same order in the output list as they were in the input list.
+-/
+theorem mergeSort_stable {l : List α} :
+    let stable_le := fun a b => if le a.2 b.2 then if le b.2 a.2 then a.1 ≤ b.1 else true else false
+    (mergeSort stable_le l.enum).map (·.2) = mergeSort le l := by
+  dsimp [stable_le]
+  rw [mergeSort_eq_naiveMergeSort, mergeSort_eq_naiveMergeSort]
+  erw [naiveMergeSort_stable] -- `erw` here to make the `stable_le` definitions match
 
 end List
+
+open List
+
+-- #time
+-- #eval (mergeSort (· ≤ ·) (iota (10^7))).length
